LabelMorph...음, 더 잘 정의된 것 같다!

src/lean/Nemonuri/Study/StanfordOnline/Compilers/Introduction/Basic.lean
@@ -1,6 +1,8 @@
 module
 
 public import Cslib.Foundations.Semantics.LTS.Basic
+public import Cslib.Foundations.Semantics.LTS.LTSCat.Basic
+public import Mathlib.Data.SetLike.Basic
 
 public section public_s
 @[expose] section expose_s
@@ -9,6 +11,7 @@ set_option autoImplicit false
 
 namespace Nemonuri.Study.StanfordOnline.Compilers
 
+/-
 universe u v
 
 structure State (St: Type u) where val: St
@@ -16,8 +19,42 @@ structure State (St: Type u) where val: St
 structure Label (La: Type v) where val: La
 
 def LTS (St: Type u) (La: Type v) := Cslib.LTS (State St) (Label La)
+-/
+
+universe us ul
+
+
+class LabelMorph (LabelA LabelB: Type _)
+  extends
+    SetLike LabelA (List (Option LabelB))
+
+
+/-
+instance (priority := low) (Label1 Label2: Type ul) : LabelMap Label1 Label2 where
+  labelMap _ := .none
+-/
+
+--def LabelMap.toMorphism {Label1 Label2 State} (inst: LabelMap Label1 Label2)
+/-
+def LabelMap.mapLTS {St} (La1 La2) [LabelMap La1 La2] (lts: Cslib.LTS St La1) : Cslib.LTS St (Option La2) :=
+  { Tr st1 la2? st2 :=
+      ∀(la1: La1), ((LabelMap.labelMap la1) = la2?) → (la2?.isSome) → (lts.Tr st1 la1 st2) }
+-/
 
 end Nemonuri.Study.StanfordOnline.Compilers
+
+/-
+open Nemonuri.Study.StanfordOnline.Compilers in
+def Cslib.LTS.mapByLabelMap {St La1} (lts: Cslib.LTS St La1) La2 [LabelMap La1 La2] : Cslib.LTS St (Option La2) :=
+  { Tr st1 la2? st2 :=
+      ∀(la1: La1), ((LabelMap.labelMap la1) = la2?) → (la2?.isSome) → (lts.Tr st1 la1 st2) }
+-/
+
+open Nemonuri.Study.StanfordOnline.Compilers in
+def Cslib.LTS.mapBySetLike {St LaB} (ltsB: Cslib.LTS St LaB) LaA [LabelMorph LaA LaB] : Cslib.LTS St LaA :=
+  { Tr st1 la st2 := ∀lb, (lb ∈ SetLike.coe la) → ltsB.withIdle.MTr st1 lb st2 }
+
+
 
 end expose_s
 end public_s
